src/SemSmall.v
@@ -1,0 +1,244 @@
+Require Import Bool List String.
+Require Import Lib.Struct Lib.Word Lib.CommonTactics Lib.FMap.
+Require Import Syntax.
+Require Export SemanticsExprAction Semantics.
+
+Set Implicit Arguments.
+
+Section GivenModule.
+  Variable m: Modules.
+  Variable oldRegs: RegsT.
+
+  Definition UpdatesT := RegsT.
+
+  Inductive SemActionSmall:
+    forall k, ActionT type k -> RegsT -> MethsT -> type k -> Prop :=
+  | SASMCallExt
+      meth s (marg: Expr type (SyntaxKind (arg s)))
+      (mret: type (ret s))
+      retK (fret: type retK)
+      (cont: type (ret s) -> ActionT type retK)
+      (HNotIn: ~ In meth (getDefs m))
+      newRegs (calls: MethsT) acalls
+      (HAcalls: acalls = M.add meth (existT _ _ (evalExpr marg, mret)) calls)
+      (HSemAction: SemActionSmall (cont mret) newRegs calls fret):
+      SemActionSmall (MCall meth s marg cont) newRegs acalls fret
+  | SASMCallInt
+      meth methBody
+      (marg: Expr type (SyntaxKind (arg (projT1 methBody))))
+      (mret: type (ret (projT1 methBody)))
+      retK (fret: type retK)
+      (cont: type (ret (projT1 methBody)) -> ActionT type retK)
+      (HIn: In (meth :: methBody)%struct (getDefsBodies m))
+      cnewRegs ccalls
+      (HCallee: SemActionSmall ((projT2 methBody) type (evalExpr marg))
+                               cnewRegs ccalls mret)
+      newRegs (calls: MethsT)
+      (HSemAction: SemActionSmall (cont mret) newRegs calls fret):
+      SemActionSmall (MCall meth (projT1 methBody) marg cont)
+                     (M.union cnewRegs newRegs) (M.union ccalls calls) fret
+  | SASLet
+      k (e: Expr type k) retK (fret: type retK)
+      (cont: fullType type k -> ActionT type retK) newRegs calls
+      (HSemActionSmall: SemActionSmall (cont (evalExpr e)) newRegs calls fret):
+      SemActionSmall (Let_ e cont) newRegs calls fret
+  | SASReadReg
+      (r: string) regT (regV: fullType type regT)
+      retK (fret: type retK) (cont: fullType type regT -> ActionT type retK)
+      newRegs calls
+      (HRegVal: M.find r oldRegs = Some (existT _ regT regV))
+      (HSemActionSmall: SemActionSmall (cont regV) newRegs calls fret):
+      SemActionSmall (ReadReg r _ cont) newRegs calls fret
+  | SASWriteReg
+      (r: string) k
+      (e: Expr type k)
+      retK (fret: type retK)
+      (cont: ActionT type retK) newRegs calls anewRegs
+      (HANewRegs: anewRegs = M.add r (existT _ _ (evalExpr e)) newRegs)
+      (HSemActionSmall: SemActionSmall cont newRegs calls fret):
+      SemActionSmall (WriteReg r e cont) anewRegs calls fret
+  | SASIfElseTrue
+      (p: Expr type (SyntaxKind Bool)) k1
+      (a: ActionT type k1)
+      (a': ActionT type k1)
+      (r1: type k1)
+      k2 (cont: type k1 -> ActionT type k2)
+      newRegs1 newRegs2 calls1 calls2 (r2: type k2)
+      (HTrue: evalExpr p = true)
+      (HAction: SemActionSmall a newRegs1 calls1 r1)
+      (HSemActionSmall: SemActionSmall (cont r1) newRegs2 calls2 r2)
+      unewRegs ucalls
+      (HUNewRegs: unewRegs = M.union newRegs1 newRegs2)
+      (HUCalls: ucalls = M.union calls1 calls2):
+      SemActionSmall (IfElse p a a' cont) unewRegs ucalls r2
+  | SASIfElseFalse
+      (p: Expr type (SyntaxKind Bool)) k1
+      (a: ActionT type k1)
+      (a': ActionT type k1)
+      (r1: type k1)
+      k2 (cont: type k1 -> ActionT type k2)
+      newRegs1 newRegs2 calls1 calls2 (r2: type k2)
+      (HFalse: evalExpr p = false)
+      (HAction: SemActionSmall a' newRegs1 calls1 r1)
+      (HSemActionSmall: SemActionSmall (cont r1) newRegs2 calls2 r2)
+      unewRegs ucalls
+      (HUNewRegs: unewRegs = M.union newRegs1 newRegs2)
+      (HUCalls: ucalls = M.union calls1 calls2):
+      SemActionSmall (IfElse p a a' cont) unewRegs ucalls r2
+  | SASAssertTrue
+      (p: Expr type (SyntaxKind Bool)) k2
+      (cont: ActionT type k2) newRegs2 calls2 (r2: type k2)
+      (HTrue: evalExpr p = true)
+      (HSemActionSmall: SemActionSmall cont newRegs2 calls2 r2):
+      SemActionSmall (Assert_ p cont) newRegs2 calls2 r2
+  | SASReturn
+      k (e: Expr type (SyntaxKind k)) evale
+      (HEvalE: evale = evalExpr e):
+      SemActionSmall (Return e) (M.empty _) (M.empty _) evale.
+
+  Theorem inversionSemActionSmall
+          k a news calls retC
+          (evalA: @SemActionSmall k a news calls retC):
+    match a with
+    | MCall meth s e c =>
+      (In meth (getDefs m) /\
+       exists methBody mret cnewRegs ccalls nnewRegs ncalls
+              (Hsig: s = projT1 methBody),
+         In (meth :: methBody)%struct (getDefsBodies m) /\
+         SemActionSmall ((projT2 methBody) type
+                                           match Hsig with
+                                             eq_refl => (evalExpr e)
+                                           end) cnewRegs ccalls mret /\
+         SemActionSmall (c (match eq_sym Hsig with eq_refl => mret end)) nnewRegs ncalls retC /\
+         news = M.union cnewRegs nnewRegs /\
+         calls = M.union ccalls ncalls) \/
+      (~ In meth (getDefs m) /\
+       exists mret pcalls,
+         SemActionSmall (c mret) news pcalls retC /\
+         calls = M.add meth (existT _ _ (evalExpr e, mret)) pcalls)
+    | Let_ _ e cont =>
+      SemActionSmall (cont (evalExpr e)) news calls retC
+    | ReadReg r k c =>
+      exists rv,
+      M.find r oldRegs = Some (existT _ k rv) /\
+      SemActionSmall (c rv) news calls retC
+    | WriteReg r _ e a =>
+      exists pnews,
+      SemActionSmall a pnews calls retC /\
+      news = M.add r (existT _ _ (evalExpr e)) pnews
+    | IfElse p _ aT aF c =>
+      exists news1 calls1 news2 calls2 r1,
+      match evalExpr p with
+      | true =>
+        SemActionSmall aT news1 calls1 r1 /\
+        SemActionSmall (c r1) news2 calls2 retC /\
+        news = M.union news1 news2 /\
+        calls = M.union calls1 calls2
+      | false =>
+        SemActionSmall aF news1 calls1 r1 /\
+        SemActionSmall (c r1) news2 calls2 retC /\
+        news = M.union news1 news2 /\
+        calls = M.union calls1 calls2
+      end
+    | Assert_ e c =>
+      SemActionSmall c news calls retC /\
+      evalExpr e = true
+    | Return e =>
+      retC = evalExpr e /\
+      news = M.empty _ /\
+      calls = M.empty _
+    end.
+  Proof.
+    destruct evalA; eauto; repeat eexists.
+    - right; repeat eexists; eauto.
+    - left; split.
+      + unfold getDefs, namesOf in *.
+        replace meth with (attrName (meth :: methBody)%struct) by reflexivity.
+        apply in_map; auto.
+      + repeat eexists; eauto.
+        * instantiate (1:= mret).
+          instantiate (1:= eq_refl).
+          simpl; auto.
+        * simpl; auto.
+    - destruct (evalExpr p); eauto; try discriminate.
+    - destruct (evalExpr p); eauto; try discriminate.
+  Qed.
+
+  Inductive SubstepSmall: UpdatesT -> LabelT -> Prop :=
+  | SSSEmptyRule:
+      SubstepSmall (M.empty _) emptyRuleLabel
+  | SSSEmptyMeth:
+      SubstepSmall (M.empty _) emptyMethLabel
+  | SSSRule:
+      forall k (a: Action Void)
+             (HInRules: List.In {| attrName := k; attrType := a |} (getRules m))
+             u cs (HAction: SemActionSmall (a type) u cs WO),
+        SubstepSmall u {| annot := Some (Some k);
+                          defs := M.empty _;
+                          calls := cs |}
+  | SSSMeth:
+      forall (f: DefMethT)
+             (HIn: In f (getDefsBodies m))
+             (HNotIn: ~ In (attrName f) (getCalls m))
+             u cs argV retV
+             (HAction: SemActionSmall ((projT2 (attrType f)) type argV) u cs retV),
+        SubstepSmall u {| annot := None;
+                          defs := M.add (attrName f) (existT _ _ (argV, retV)) (M.empty _);
+                          calls := cs |}.
+
+  Definition CanCombineLabels (u1 u2: UpdatesT) (l1 l2: LabelT) :=
+    M.Disj u1 u2 /\
+    M.Disj (defs l1) (defs l2) /\
+    M.Disj (calls l1) (calls l2) /\
+    match annot l1, annot l2 with
+    | Some _, Some _ => False
+    | _, _ => True
+    end.
+
+  Inductive SubstepsSmall: UpdatesT -> LabelT -> Prop :=
+  | SSSNil:
+      SubstepsSmall (M.empty _) emptyMethLabel
+  | SSSCons:
+      forall pu pl,
+        SubstepsSmall pu pl ->
+        forall nu nl,
+          CanCombineLabels pu nu pl nl ->
+          SubstepSmall nu nl ->
+          SubstepsSmall (M.union pu nu) (mergeLabel nl pl).
+
+  Inductive StepSmall: UpdatesT -> LabelT -> Prop :=
+  | StepSmallIntro: forall u l (HSubSteps: SubstepsSmall u l),
+      StepSmall u l.
+
+End GivenModule.
+
+Ltac invertActionSmall H := apply inversionSemActionSmall in H; simpl in H; dest; try subst.
+Ltac invertActionSmallFirst :=
+  match goal with
+  | [H: SemActionSmall _ _ _ _ _ _ |- _] => invertActionSmall H
+  end.
+Ltac invertActionSmallRep :=
+  repeat
+    match goal with
+    | [H: SemActionSmall _ _ _ _ _ _ |- _] => invertActionSmall H
+    | [H: if ?c
+          then
+            SemActionSmall _ _ _ _ _ _ /\ _ /\ _ /\ _
+          else
+            SemActionSmall _ _ _ _ _ _ /\ _ /\ _ /\ _ |- _] =>
+      let ic := fresh "ic" in
+      (remember c as ic; destruct ic; dest; subst)
+    end.
+
+Section Facts.
+
+  Lemma stepSmall_consistent:
+    forall m o u l,
+      Step m o u l <-> StepSmall m o u l.
+  Proof.
+    admit.
+  Qed.
+
+End Facts.
+
+
